SatSolver.lean
@@ -10,8 +10,8 @@ def parseDimacs (n : Nat) [NeZero n] (lines : List String) : Std.Sat.CNF (Fin n)
            | some 0 => none
            | some i => some (
               if i > 0
-              then ⟨⟨i.natAbs % n, by refine Nat.mod_lt i.natAbs ?_; simp only [gt_iff_lt]; exact Nat.pos_of_neZero n⟩, true⟩
-              else ⟨⟨i.natAbs % n, by refine Nat.mod_lt i.natAbs ?_; simp only [gt_iff_lt]; exact Nat.pos_of_neZero n⟩, false⟩
+              then ⟨⟨i.natAbs % n, by refine Nat.mod_lt i.natAbs ?_; exact Nat.pos_of_neZero n⟩, true⟩
+              else ⟨⟨i.natAbs % n, by refine Nat.mod_lt i.natAbs ?_; exact Nat.pos_of_neZero n⟩, false⟩
             )
            | none   => none)
        )
